test/Append.v
@@ -354,6 +354,11 @@ Module SepContracts.
     (AssertionKit ExampleTermKit ExampleProgramKit).
     Export ExampleProgramKit.
 
+    Definition 𝑷 := Empty_set.
+    Definition 𝑷_Ty : 𝑷 -> Ctx Ty := fun p => match p with end.
+    Definition 𝑷_inst (p : 𝑷) : abstract Lit (𝑷_Ty p) Prop := match p with end.
+    Instance 𝑷_eq_dec : EqDec 𝑷 := fun p => match p with end.
+
     Definition 𝑯 := Predicate.
     Definition 𝑯_Ty (p : 𝑯) : Ctx Ty :=
       match p with
