test/Example.v
@@ -359,6 +359,11 @@ Module SepContracts.
     (AssertionKit ExampleTermKit ExampleProgramKit).
     Export ExampleProgramKit.
 
+    Definition 𝑷 := Empty_set.
+    Definition 𝑷_Ty : 𝑷 -> Ctx Ty := fun p => match p with end.
+    Definition 𝑷_inst (p : 𝑷) : abstract Lit (𝑷_Ty p) Prop := match p with end.
+    Instance 𝑷_eq_dec : EqDec 𝑷 := fun p => match p with end.
+
     Definition 𝑯 := Empty_set.
     Definition 𝑯_Ty : 𝑯 -> Ctx Ty := fun p => match p with end.
     Instance 𝑯_eq_dec : EqDec 𝑯 := fun p => match p with end.
