theories/Symbolic/Mutator.v
@@ -674,6 +674,8 @@ Module Mutators
 
     Definition simplify_formula {Σ} (fml : Formula Σ) (k : List Formula Σ) : option (List Formula Σ) :=
       match fml with
+      (* TODO: partial evaluation of ts *)
+      | formula_user p ts => Some (cons fml k)
       | formula_bool t    => simplify_formula_bool (peval t) k
       | formula_prop ζ P  => Some (cons fml k)
       | formula_ge t1 t2  => simplify_formula_bool (peval (term_binop binop_ge t1 t2)) k
@@ -771,6 +773,7 @@ Module Mutators
         (simplify_formula fml k).
     Proof.
       destruct fml; cbn - [peval].
+      - admit.
       - generalize (simplify_formula_bool_spec (peval t) k).
         apply optionspec_monotonic; cbn; intros; specialize (H ι);
           now rewrite (peval_sound t) in H.
@@ -799,7 +802,7 @@ Module Mutators
         apply optionspec_monotonic; cbn; intros; specialize (H ι);
           now rewrite (peval_sound t1), (peval_sound t2) in H.
       - constructor. intros ι. now rewrite inst_pathcondition_cons.
-    Qed.
+    Admitted.
 
     Lemma simplify_formulas_spec {Σ} (fmls k : List Formula Σ) :
       OptionSpec
